Additions: - induction principle for statements. - equality testing (including annotations) for expressions and statements. - equality testing (excluding statements) for statements.

ott/coq/AilSyntax_proof.v
@@ -44,7 +44,6 @@ Proof.
   my_auto.
 Qed.
 
-
 Definition expression_nrect
          {A}
          (P : expression' A -> Type)
@@ -93,6 +92,37 @@ with g e : Q e :=
   end
 for g.
 
+
+Lemma eq_expression_correct {A : Set} {eq_A} :
+  (forall x y : A, boolSpec (eq_A x y) (x = y)) ->
+  forall (x y : expression A), boolSpec (eq_expression eq_A x y) (x = y).
+Proof.
+  intros eq_A_correct.
+  apply (expression_nrect (fun x => forall y, boolSpec (eq_expression' eq_A x y) (x = y))
+                          (fun x => forall y, boolSpec (eq_expression  eq_A x y) (x = y))
+                          (fun x => forall y, boolSpec (eq_arguments   eq_A x y) (x = y)));
+  intros; destruct y;
+  unfold_goal; simpl;
+  match goal with
+  | |- context[eq_arguments_aux _ _ ?es1 ?es2] => fold (eq_arguments eq_A es1 es2)
+  | _ => idtac
+  end; unfold andb;
+  repeat match goal with
+  | |- eq_unaryOperator ?x ?y = _ -> _ => case_fun (eq_unaryOperator_correct x y)
+  | |- eq_binaryOperator ?x ?y = _ -> _ => case_fun (eq_binaryOperator_correct x y)
+  | |- eq_arithmeticOperator ?x ?y = _ -> _ => case_fun (eq_arithmeticOperator_correct x y)
+  | |- eq_ctype ?x ?y = _ -> _ => case_fun (eq_ctype_correct x y)
+  | |- eq_identifier ?x ?y = _ -> _ => case_fun (eq_identifier_correct x y)
+  | |- eq_qualifiers ?x ?y = _ -> _ => case_fun (eq_qualifiers_correct x y)
+  | |- eq_constant ?x ?y = _ -> _ => case_fun (eq_constant_correct x y)
+  | |- eq_A ?x ?y = _ -> _ => case_fun (eq_A_correct x y)
+  | IH : forall _, boolSpec (eq_expression _ ?x _) _|- eq_expression _ ?x ?y = _ -> _ => case_fun (IH y)
+  | IH : forall _, boolSpec (eq_expression' _ ?x _) _|- eq_expression' _ ?x ?y = _ -> _ => case_fun (IH y)
+  | IH : forall _, boolSpec (eq_arguments _ ?x _) _|- eq_arguments _ ?x ?y = _ -> _ => case_fun (IH y)
+  | _ => context_destruct
+  end; now my_auto.
+Qed.
+
 Lemma equiv_expression_correct {A} :
   forall (x y : expression A), boolSpec (equiv_expression x y) (equivExpression x y).
 Proof.
@@ -116,6 +146,148 @@ Proof.
   | IH : forall _, boolSpec (equiv_expression ?x _) _|- equiv_expression ?x ?y = _ -> _ => case_fun (IH y)
   | IH : forall _, boolSpec (equiv_expression' ?x _) _|- equiv_expression' ?x ?y = _ -> _ => case_fun (IH y)
   | IH : forall _, boolSpec (equiv_arguments ?x _) _|- equiv_arguments ?x ?y = _ -> _ => case_fun (IH y)
+  | _ => context_destruct
+  end; now my_auto.
+Qed.
+
+Lemma eq_bindings_correct x y :
+  boolSpec (eq_bindings x y) (x = y).
+Proof.
+  apply (eq_list_correct
+           (eq_pair_correct eq_identifier_correct
+                            (eq_pair_correct
+                               eq_qualifiers_correct
+                               eq_ctype_correct))
+        ).
+Qed.
+
+Lemma eq_declaration_correct {A : Set} {eq_A} :
+  (forall x y : A, boolSpec (eq_A x y) (x = y)) ->
+  forall x y, boolSpec (eq_declaration eq_A x y) (x = y).
+Proof.
+  intros eq_A_correct.
+  apply (eq_list_correct (eq_pair_correct eq_identifier_correct (eq_expression_correct eq_A_correct))).
+Qed.
+
+Fixpoint equiv_declaration_correct {A : Set} (x y : list (identifier * expression A)) :
+    boolSpec (equiv_declaration x y) (equivDeclaration x y).
+Proof.
+  unfold_goal.
+  destruct x, y; simpl; unfold andb; intuition;
+  repeat match goal with
+  | |- eq_identifier ?x ?y = _ -> _ => case_fun (eq_identifier_correct x y)
+  | |- equiv_expression ?x ?y = _ -> _ => case_fun (equiv_expression_correct x y)
+  | |- equiv_declaration ?x ?y = _ -> _ => case_fun (equiv_declaration_correct A x y)
+  | _ => context_destruct
+  end; my_auto.
+Qed.
+
+Definition statement_nrect
+           {A B}
+           (P : statement' A B -> Type)
+           (Q : statement A B  -> Type)
+           (R : list (statement A B) -> Type)
+
+           (HSkip : P Skip)
+           (HExpression : forall {e}, P (Expression e))
+           (HBlock : forall {b} {ss}, R ss -> P (Block b ss))
+           (HIf : forall {e} {s1 s2}, Q s1 -> Q s2 -> P (If e s1 s2))
+           (HWhile : forall {e} {s}, Q s -> P (While e s))
+           (HDo : forall {s} {e}, Q s -> P (Do s e))
+           (HBreak : P Break)
+           (HContinue : P Continue)
+           (HReturnVoid : P ReturnVoid)
+           (HReturn : forall {e}, P (Return e))
+           (HSwitch : forall {e} {s}, Q s -> P (Switch e s))
+           (HCase : forall {ic} {s}, Q s -> P (Case ic s))
+           (HDefault : forall {s}, Q s -> P (Default s))
+           (HLabel : forall {v} {s}, Q s -> P (Label v s))
+           (HGoto : forall {v}, P (Goto v))
+           (HDeclaration : forall {d}, P (Declaration d))
+           (Hnil : R nil)
+           (Hcons : forall {s} {ss}, Q s -> R ss -> R (s :: ss))
+           (HAnnotatedStatement : forall {a} {s}, P s -> Q (AnnotatedStatement a s)) :
+  forall s : statement A B, Q s
+:=
+  fix f s : P s :=
+    match s return P s with
+    | Skip => HSkip
+    | Expression _ => HExpression
+    | Block _ _ =>
+        let fix h ss : R ss :=
+          match ss return R ss with
+          | nil     => Hnil
+          | s :: ss => Hcons (g s) (h ss)
+          end in
+        HBlock (h _)
+    | If _ _ _ => HIf (g _) (g _)
+    | While _ _ => HWhile (g _)
+    | Do _ _ => HDo (g _)
+    | Break => HBreak
+    | Continue => HContinue
+    | ReturnVoid => HReturnVoid
+    | Return _ => HReturn
+    | Switch _ _ => HSwitch (g _)
+    | Case _ _ => HCase (g _)
+    | Default _ => HDefault (g _)
+    | Label _ _ => HLabel (g _)
+    | Goto _ => HGoto
+    | Declaration _ => HDeclaration
+    end
+with g s : Q s :=
+  match s return Q s with
+  | AnnotatedStatement _ _ => HAnnotatedStatement (f _)
+  end
+for g.
+
+Lemma equiv_statement_correct {A B} :
+  forall (x y : statement A B), boolSpec (equiv_statement x y) (equivStatement x y).
+Proof.
+  apply (statement_nrect (fun x => forall y, boolSpec (equiv_statement' x y) (equivStatement' x y))
+                         (fun x => forall y, boolSpec (equiv_statement  x y) (equivStatement  x y))
+                         (fun x => forall y, boolSpec (equiv_block      x y) (equivBlock      x y)));
+  intros;
+  unfold_goal; destruct y; simpl; unfold andb;
+  repeat match goal with
+  | |- eq_ctype ?x ?y = _ -> _ => case_fun (eq_ctype_correct x y)
+  | |- eq_identifier ?x ?y = _ -> _ => case_fun (eq_identifier_correct x y)
+  | |- eq_qualifiers ?x ?y = _ -> _ => case_fun (eq_qualifiers_correct x y)
+  | |- eq_bindings ?x ?y = _ -> _ => case_fun (eq_bindings_correct x y)
+  | |- eq_integerConstant ?x ?y = _ -> _ => case_fun (eq_integerConstant_correct x y)
+  | |- equiv_declaration ?x ?y = _ -> _ => case_fun (equiv_declaration_correct x y)
+  | |- equiv_expression ?x ?y = _ -> _ => case_fun (equiv_expression_correct x y)
+  | IH : forall _, boolSpec (equiv_statement ?x _) _|- equiv_statement ?x ?y = _ -> _ => case_fun (IH y)
+  | IH : forall _, boolSpec (equiv_statement' ?x _) _|- equiv_statement' ?x ?y = _ -> _ => case_fun (IH y)
+  | |- equiv_block_aux _ ?x ?y = _ -> _ => fold (equiv_block x y)
+  | IH : forall _, boolSpec (equiv_block ?x _) _|- equiv_block ?x ?y = _ -> _ => case_fun (IH y)
+  | _ => context_destruct
+  end; now my_auto.
+Qed.
+
+Lemma eq_statement_correct {A B : Set} {eq_A} {eq_B} :
+  (forall x y : A, boolSpec (eq_A x y) (x = y)) ->
+  (forall x y : B, boolSpec (eq_B x y) (x = y)) ->
+  forall (x y : statement A B), boolSpec (eq_statement eq_A eq_B x y) (x = y).
+Proof.
+  intros eq_A_correct eq_B_correct.
+  apply (statement_nrect (fun x => forall y, boolSpec (eq_statement' eq_A eq_B x y) (x = y))
+                         (fun x => forall y, boolSpec (eq_statement  eq_A eq_B x y) (x = y))
+                         (fun x => forall y, boolSpec (eq_block      eq_A eq_B x y) (x = y)));
+  intros;
+  unfold_goal; destruct y; simpl; unfold andb;
+  repeat match goal with
+  | |- eq_A ?x ?y = _ -> _ => case_fun (eq_A_correct x y)
+  | |- eq_ctype ?x ?y = _ -> _ => case_fun (eq_ctype_correct x y)
+  | |- eq_identifier ?x ?y = _ -> _ => case_fun (eq_identifier_correct x y)
+  | |- eq_qualifiers ?x ?y = _ -> _ => case_fun (eq_qualifiers_correct x y)
+  | |- eq_bindings ?x ?y = _ -> _ => case_fun (eq_bindings_correct x y)
+  | |- eq_integerConstant ?x ?y = _ -> _ => case_fun (eq_integerConstant_correct x y)
+  | |- eq_declaration eq_B ?x ?y = _ -> _ => case_fun (eq_declaration_correct eq_B_correct x y)
+  | |- eq_expression _ ?x ?y = _ -> _ => case_fun (eq_expression_correct eq_B_correct x y)
+  | IH : forall _, boolSpec (eq_statement _ _ ?x _) _|- eq_statement _ _ ?x ?y = _ -> _ => case_fun (IH y)
+  | IH : forall _, boolSpec (eq_statement' _ _ ?x _) _|- eq_statement' _ _ ?x ?y = _ -> _ => case_fun (IH y)
+  | |- eq_block_aux _ _ _ ?x ?y = _ -> _ => fold (eq_block eq_A eq_B x y)
+  | IH : forall _, boolSpec (eq_block _ _ ?x _) _|- eq_block _ _ ?x ?y = _ -> _ => case_fun (IH y)
   | _ => context_destruct
   end; now my_auto.
 Qed.
